Switch to a style where padded ciphers are kept in the table, and where the post-condition of decrypt is uniform via a new xor operation

src/Model.PNE.fst
@@ -79,9 +79,9 @@ let encrypt #j #u st #l n s =
     let (| u, p |) = st <: model_state j in
     let log = !*p in
     assert (log == table st h0);
-    let cipher: pne_cipher l = random l, random_bits () in
+    let cipher: pne_cipherpad = random 5, random_bits () in
     p *= Seq.snoc log (Entry s #l n cipher);
-    cipher
+    clip_cipherpad cipher l
   else
     let open QUIC.Spec.Lemmas in
     let pn, bits = PNEPlainPkg?.repr u.plain j l n in
@@ -89,29 +89,39 @@ let encrypt #j #u st #l n s =
     let alg = (fst (st <: unsafe_state j)).calg in
     encrypt_spec alg l pn bits s k
 
+#push-options "--fuel 1"
 let snoc_find #a (s: Seq.seq a) (f: a -> bool) (x: a): Lemma
-  (requires f x)
-  (ensures Some? (FStar.Seq.(find_l f (snoc s x))))
+  (requires f x /\ None? FStar.Seq.(find_l f s))
+  (ensures FStar.Seq.(find_l f (snoc s x)) == Some x)
 =
-  admit ()
+  assert (Seq.snoc s x `Seq.equal` Seq.append s (Seq.create 1 x));
+  Seq.find_append_none s (Seq.create 1 x) f;
+  ()
+#pop-options
 
 let decrypt #j #u st cp s =
   if is_safe j then
     let (| info, p |) = st <: model_state j in
     let log = !*p in
-    match Seq.find_l (sample_cipherpad_filter s cp) log with
+    match Seq.find_l (sample_filter u s) log with
+    | Some (Entry _ #l' n' c') ->
+        // The sample is present in the table, cipher may or may not match, it's
+        // up to the caller to prove that when there's a match (i.e. c' == cp)
+        // then c'' == zeroes which then entails that the returns value is the
+        // plaintext that was in the table
+        let c'' = c' `xor_cipherpad` cp in
+        PNEPlainPkg?.xor u.plain j l' n' c''
     | None ->
+        // Need to add into the table:
         let bits = random_bits () in
         let l = LowParse.BitFields.get_bitfield bits 0 2 + 1 in
-        let plain = random l in
-        let n = PNEPlainPkg?.mk u.plain j l plain bits in
-        p *= Seq.snoc log (Entry s #l n (clip_cipherpad cp l));
-        let h1 = ST.get () in
-        snoc_find log (sample_filter u s) (Entry s #l n (clip_cipherpad cp l));
-        (| l, n |)
-    | Some (Entry _ #l' n' c') ->
-        assert (c' == clip_cipherpad cp l');
-        (| l', n' |)
+        let c' = random 5, bits in
+        // let n' = clip_cipherpad (c' `xor_cipherpad` cp) l in
+        let n = PNEPlainPkg?.mk u.plain j l (random l) bits in
+        let new_log = Seq.snoc log (Entry s #l n c') in
+        p *= new_log;
+        snoc_find log (sample_filter u s) (Entry s #l n c');
+        PNEPlainPkg?.xor u.plain j l n (c' `xor_cipherpad` cp)
   else
     let info, k = st <: unsafe_state j in
     decrypt_spec info.calg (fst cp) (snd cp) k s
